@prefix : <http://www.w3.org/ns/td#> .
@prefix dc: <http://purl.org/dc/elements/1.1/> .
@prefix vs: <http://www.w3.org/2003/06/sw-vocab-status/ns#> .
@prefix owl: <http://www.w3.org/2002/07/owl#> .
@prefix rdf: <http://www.w3.org/1999/02/22-rdf-syntax-ns#> .
@prefix xml: <http://www.w3.org/XML/1998/namespace> .
@prefix xsd: <http://www.w3.org/2001/XMLSchema#> .
@prefix foaf: <http://xmlns.com/foaf/0.1/> .
@prefix prov: <http://www.w3.org/ns/prov#> .
@prefix rdfs: <http://www.w3.org/2000/01/rdf-schema#> .
@prefix vann: <http://purl.org/vocab/vann/> .
@prefix dcterms: <http://purl.org/dc/terms/> .

<http://www.w3.org/ns/td#> rdf:type owl:Ontology ;
                           
                           owl:versionInfo "0.0.1" ;
                           
                           vann:preferredNamespacePrefix "td" ;
                           
                           dc:title "Ontology model for Web of Things"@en ;
                           
                           rdfs:comment "This ontology aims to model the Web of Things domain according to the W3C Interest Group (http://w3c.github.io/wot/)"@en ;
                           
                           vann:preferredNamespaceUri "http://www.w3.org/ns/td#" ;
                           
                           dcterms:license <http://purl.org/NET/rdflicense/cc-by4.0> ;
                           
                           dcterms:creator <http://purl.org/net/mpoveda> ,
                                           <http://www.garcia-castro.com/foaf.rdf#me> ;
                           
                           dcterms:contributor <http://www.oeg-upm.net/index.php/en/universitystaff/402-fserena/> ;
                           
                           dc:publisher <https://www.w3.org/WoT/WG/> .


#################################################################
#
#    Annotation properties
#
#################################################################


###  http://www.w3.org/2003/06/sw-vocab-status/ns#term_status

vs:term_status rdf:type owl:AnnotationProperty .





#################################################################
#
#    Object Properties
#
#################################################################


###  http://www.w3.org/ns/td#actions

:actions rdf:type owl:ObjectProperty ;
         
         rdfs:label "actions" ;
         
         rdfs:comment "Keeps all Action-based interaction patterns of the Thing."@en ;
         
         rdfs:range :Action ;
         
         rdfs:domain :Thing .



###  http://www.w3.org/ns/td#events

:events rdf:type owl:ObjectProperty ;
        
        rdfs:label "events" ;
        
        rdfs:comment "Keeps all Event-based interaction patterns of the Thing."@en .



###  http://www.w3.org/ns/td#forms

:forms rdf:type owl:ObjectProperty ;
       
       rdfs:label "forms" ;
       
       rdfs:comment "Indicates one or more endpoints from which an interaction pattern is accessible"@en .



###  http://www.w3.org/ns/td#input

:input rdf:type owl:ObjectProperty ;
       
       rdfs:label "input" ;
       
       rdfs:comment "Link to the n-ary class that allows the declaration of the accepted data type of an action."@en ;
       
       rdfs:range :Property ;
       
       rdfs:domain :Thing .



###  http://www.w3.org/ns/td#items

:items rdf:type owl:ObjectProperty ;
       
       rdfs:label "items" ;
       
       rdfs:comment "Used to define characteristics of an array."@en ;
       
       rdfs:range :Property ;
       
       rdfs:domain :Thing .



###  http://www.w3.org/ns/td#links

:links rdf:type owl:ObjectProperty ;
       
       rdfs:label "links" ;
       
       rdfs:comment "Provides Web links to arbitrary resources that relate to the specified Thing Description."@en .



###  http://www.w3.org/ns/td#objectSchemaProperties

:objectSchemaProperties rdf:type owl:ObjectProperty ;
                        
                        rdfs:label "properties" ;
                        
                        rdfs:comment "Data schema nested definitions"@en .



###  http://www.w3.org/ns/td#output

:output rdf:type owl:ObjectProperty ;
        
        rdfs:label "output" ;
        
        rdfs:comment "Link to the n-ary class that allows the declaration of the data type returned by an action."@en ;
        
        rdfs:range :Property ;
        
        rdfs:domain :Thing .



###  http://www.w3.org/ns/td#properties

:properties rdf:type owl:ObjectProperty ;
            
            rdfs:label "properties" ;
            
            rdfs:comment "Keeps all Property-based interaction patterns of the Thing."@en ;
            
            rdfs:range :Property ;
            
            rdfs:domain :Thing .



###  http://www.w3.org/ns/td#schema

:schema rdf:type owl:ObjectProperty ;
        
        rdfs:label "schema" ;
        
        rdfs:comment "Schema definition for values of the given object schema property."@en ;
        
        rdfs:range :Property .


###  http://www.w3.org/ns/td#scopes

:scope rdf:type owl:ObjectProperty ;
        
       rdfs:label "scopes" ;
        
       rdfs:comment "Array of authorization scope identifiers."@en ;
        
       rdfs:range :Thing .

###  http://www.w3.org/ns/td#security

:security rdf:type owl:ObjectProperty ;
       
       rdfs:label "security" ;
       
       rdfs:comment "Set of security configurations that must all be satisfied for access to resources at or below the annotated level."@en .

#################################################################
#
#    Data properties
#
#################################################################


###  http://www.w3.org/ns/td#alg

:alg rdf:type owl:DatatypeProperty ;
          
     rdfs:label "alg" ;
             
     rdfs:comment "Encoding, encryption, or digest algorithm (one of MD5, ES256, or ES512-256)."@en ;
             
     rdfs:range xsd:string .


###  http://www.w3.org/ns/td#anchor

:anchor rdf:type owl:DatatypeProperty ;
        
        rdfs:label "anchor" ;
        
        rdfs:comment "By default, the context of a link is the URL of the representation it is associated with, and is serialised as a URI. When present, the anchor parameter overrides this with another URI, such as a fragment of this resource, or a third resource (i.e., when the anchor value is an absolute URI)."@en .


###  http://www.w3.org/ns/td#authorizationUrl

:authorizationUrl rdf:type owl:DatatypeProperty ;
      
      rdfs:label "authorizationUrl" ;
      
      rdfs:comment "URI of the authorization server."@en ;
      
      rdfs:range xsd:anyURI .



###  http://www.w3.org/ns/td#base

:base rdf:type owl:DatatypeProperty ;
      
      rdfs:label "base"@en ;
      
      rdfs:comment "Define base URI that is valid for all defined local interaction resources. All other URIs in the TD must then be resolved using the algorithm defined in [[!RFC3986]]. This field is optional."@en ;
      
      rdfs:range xsd:anyURI .



###  http://www.w3.org/ns/td#const

:const rdf:type owl:DatatypeProperty ;
       
       rdfs:label "const" ;
       
       rdfs:comment "Provides a constant value."@en ;
       
       rdfs:range rdfs:Literal .



###  http://www.w3.org/ns/td#description

:description rdf:type owl:DatatypeProperty ;
             
             rdfs:label "description" ;
             
             rdfs:comment "Provides additional (human) readable information."@en ;
             
             rdfs:range xsd:string .



###  http://www.w3.org/ns/td#enum

:enum rdf:type owl:DatatypeProperty ;
      
      rdfs:label "enum" ;
      
      rdfs:comment "Restricted set of values provided as array."@en ;
      
      rdfs:range rdfs:Literal .



###  http://www.w3.org/ns/td#flow

:flow rdf:type owl:DatatypeProperty ;
             
      rdfs:label "flow" ;
             
      rdfs:comment "Authorization flow (one of implicit, password, client, or code)"@en ;
             
      rdfs:range xsd:string .



###  http://www.w3.org/ns/td#href

:href rdf:type owl:DatatypeProperty ,
               owl:FunctionalProperty ;
      
      rdfs:label "href" ;
      
      rdfs:comment "URI of the endpoint where an interaction pattern is provided"@en ;
      
      rdfs:range xsd:anyURI .



###  http://www.w3.org/ns/td#id

:id rdf:type owl:DatatypeProperty ;
    
    rdfs:label "id" ;
    
    rdfs:comment "Defines unique URI (includes also URNs) ID of the Thing."@en ;
    
    rdfs:range xsd:anyURI .



###  http://www.w3.org/ns/td#in

:in rdf:type owl:DatatypeProperty ;
    
    rdfs:label "in" ;
    
    rdfs:comment "Specifies location of security authentication information (one of header, query, body, or cookie)."@en ;
    
    rdfs:range xsd:string .



###  http://www.w3.org/ns/td#format

:format rdf:type owl:DatatypeProperty ;
    
    rdfs:label "format" ;
    
    rdfs:comment "Specifies format of security authentication information (one of jwt, jwe, or jws)."@en ;
    
    rdfs:range xsd:string .


###  http://www.w3.org/ns/td#label

:label rdf:type owl:DatatypeProperty ;
       
       rdfs:label "label" ;
       
       rdfs:comment "Provides a label (e.g., display a text for UI representation) of the interaction pattern."@en ;
       
       rdfs:range xsd:string .



###  http://www.w3.org/ns/td#maxItems

:maxItems rdf:type owl:DatatypeProperty ;
          
          rdfs:label "maxItems" ;
          
          rdfs:comment "Defines the maximum number of items that have to be in the array."@en ;
          
          rdfs:range xsd:unsignedInt .



###  http://www.w3.org/ns/td#maximum

:maximum rdf:type owl:DatatypeProperty ;
         
         rdfs:label "maximum" ;
         
         rdfs:comment "Specifies a maximum numeric value. Only applicable for associated number or integer types."@en ;
         
         rdfs:seeAlso <http://schema.org/maxValue> ;
         
         rdfs:range xsd:double .



###  http://www.w3.org/ns/td#mediaType

:mediaType rdf:type owl:DatatypeProperty ;
           
           rdfs:label "mediaType" ;
           
           rdfs:comment "Assign underlying media type of the interaction pattern based on IANA (https://www.iana.org/assignments/media-types/media-types.xhtml)"@en ;
           
           rdfs:range xsd:string .



###  http://www.w3.org/ns/td#minItems

:minItems rdf:type owl:DatatypeProperty ;
          
          rdfs:label "minItems" ;
          
          rdfs:comment "Defines the minimum number of items that have to be in the array."@en ;
          
          rdfs:range xsd:unsignedInt .



###  http://www.w3.org/ns/td#minimum

:minimum rdf:type owl:DatatypeProperty ;
         
         rdfs:label "minimum" ;
         
         rdfs:comment "Specifies a minimum numeric value. Only applicable for associated number or integer types."@en ;
         
         rdfs:seeAlso <http://schema.org/minValue> ;
         
         rdfs:range xsd:double .



###  http://www.w3.org/ns/td#name

:name rdf:type owl:DatatypeProperty ;
      
      rdfs:label "name" ;
      
      rdfs:comment "Name of the Thing or interaction pattern (must be a valid keyword to be used in the scripting API)"@en ;
      
      rdfs:range xsd:string .



###  http://www.w3.org/ns/td#observable

:observable rdf:type owl:DatatypeProperty ,
                     owl:FunctionalProperty ;
            
            rdfs:label "observable" ;
            
            rdfs:comment "Indicates whether a remote servient can subscribe to (\"observe\") the Property, to receive change notifications or periodic updates (true/false)."@en ;
            
            rdfs:range xsd:boolean .


###  http://www.w3.org/ns/td#pname

:qop rdf:type owl:DatatypeProperty ;
          
     rdfs:label "pname" ;
             
     rdfs:comment "Name for query, header, or cookie parameters." ;
             
     rdfs:range xsd:string .



###  http://www.w3.org/ns/td#proxyUrl

:proxyUrl rdf:type owl:DatatypeProperty ;
      
      rdfs:label "proxyUrl" ;
      
      rdfs:comment "URI of the proxy server this security configuration provides access to.  If not given, the corresponding security configuration is for the endpoint."@en ;
      
      rdfs:range xsd:anyURI .



###  http://www.w3.org/ns/td#qop

:qop rdf:type owl:DatatypeProperty ;
          
     rdfs:label "qop" ;
             
     rdfs:comment "Quality of protection (one of auth or auth-int)." ;
             
     rdfs:range xsd:string .



###  http://www.w3.org/ns/td#refreshUrl

:refreshUrl rdf:type owl:DatatypeProperty ;
      
      rdfs:label "refreshUrl" ;
      
      rdfs:comment "URI of the refresh server"@en ;
      
      rdfs:range xsd:anyURI .



###  http://www.w3.org/ns/td#rel

:rel rdf:type owl:DatatypeProperty ;
     
     rdfs:label "rel" ;
     
     rdfs:comment """Indicates the expected result of performing the operation described by the form.

For example, the Property interaction allows get and set operations. The protocol binding may contain a form for the get operation and a different form for the set operation. The value of the \"rel\" attribute of the form indicates which form is which and allows the client to select the correct form for the oeration required"""@en ;
     
     rdfs:range xsd:string .



###  http://www.w3.org/ns/td#required

:required rdf:type owl:DatatypeProperty ;
          
          rdfs:label "required" ;
          
          rdfs:comment "Defines which members of the object type are required/mandatory."@en ;
          
          rdfs:range xsd:string .



###  http://www.w3.org/ns/td#scheme

:scheme rdf:type owl:DatatypeProperty ;
        
        rdfs:label "scheme" ;
        
        rdfs:comment "Identification of security mechanism being configured (one of basic, digest, bearer, pop, oauth2, or apikey)."@en ;
        rdfs:range xsd:string .



###  http://www.w3.org/ns/td#support

:support rdf:type owl:DatatypeProperty ;
         
         rdfs:label "support" ;
         
         rdfs:comment "Provides information about TD maintainer (e.g., author, link or telephone number to get support, etc)."@en ;

         rdfs:range xsd:string .

###  http://www.w3.org/ns/td#tokenUrl

:tokenUrl rdf:type owl:DatatypeProperty ;
      
      rdfs:label "tokenUrl" ;
      
      rdfs:comment "URI of the token server."@en ;
      
      rdfs:range xsd:anyURI .


###  http://www.w3.org/ns/td#type

:type rdf:type owl:DatatypeProperty ;
      
      rdfs:label "type" ;
      
      rdfs:comment "Assignment of JSON-based data types that are compatible with JSON Schema (one of boolean, integer, number, string, object, array, or null)." ;
      
      rdfs:range xsd:string .



###  http://www.w3.org/ns/td#writable

:writable rdf:type owl:DatatypeProperty ,
                   owl:FunctionalProperty ;
          
          rdfs:label "writable" ;
          
          rdfs:comment "Boolean value that indicates whether a property is writable (=true) or not (=false)"@en ;
          
          rdfs:range xsd:boolean .





#################################################################
#
#    Classes
#
#################################################################


###  http://www.w3.org/ns/td#Action

:Action rdf:type owl:Class ;
        
        rdfs:label "Action" ;
        
        rdfs:subClassOf [ rdf:type owl:Restriction ;
                          owl:onProperty :description ;
                          owl:allValuesFrom xsd:string
                        ] ,
                        [ rdf:type owl:Restriction ;
                          owl:onProperty :input ;
                          owl:allValuesFrom :Property
                        ] ,
                        [ rdf:type owl:Restriction ;
                          owl:onProperty :label ;
                          owl:allValuesFrom xsd:string
                        ] ,
                        [ rdf:type owl:Restriction ;
                          owl:onProperty :security ;
                          owl:allValuesFrom :SecurityScheme
                        ] ,
                        [ rdf:type owl:Restriction ;
                          owl:onProperty :scopes ;
                          owl:allValuesFrom xsd:string
                        ] ,
                        [ rdf:type owl:Restriction ;
                          owl:onProperty :forms ;
                          owl:allValuesFrom :Form
                        ] ,
                        [ rdf:type owl:Restriction ;
                          owl:onProperty :output ;
                          owl:allValuesFrom :Property
                        ] ;
        
        rdfs:comment "Actions offer functions of the Thing. These functions may manipulate the interal state of a Thing in a way that is not possible through setting Properties. Examples are changing internal state that is not exposed as Property, changing multiple Properties, changing Properties over time or with a process that shall not be disclosed. Actions may also be pure functions, that is, they do not use any internal state at all, e.g., for processing input data and returning the result directly."@en .



###  http://www.w3.org/ns/td#ArraySchema

:ArraySchema rdf:type owl:Class ;
             
             rdfs:subClassOf :DataSchema ,
                             [ rdf:type owl:Restriction ;
                               owl:onProperty :maxItems ;
                               owl:allValuesFrom xsd:unsignedInt
                             ] ,
                             [ rdf:type owl:Restriction ;
                               owl:onProperty :minItems ;
                               owl:allValuesFrom xsd:unsignedInt
                             ] ,
                             [ rdf:type owl:Restriction ;
                               owl:onProperty :items ;
                               owl:allValuesFrom :DataSchema
                             ] ;
             
             rdfs:comment "A JSON array specification (\"type\": \"array\")."@en .



###  http://www.w3.org/ns/td#BooleanSchema

:BooleanSchema rdf:type owl:Class ;
               
               rdfs:subClassOf :DataSchema ;
               
               rdfs:comment "A JSON boolean value specification (\"type\": \"boolean\")."@en .



###  http://www.w3.org/ns/td#DataSchema

:DataSchema rdf:type owl:Class ;
            
            rdfs:subClassOf [ rdf:type owl:Restriction ;
                              owl:onProperty :const ;
                              owl:allValuesFrom rdfs:Literal
                            ] ,
                            [ rdf:type owl:Restriction ;
                              owl:onProperty :type ;
                              owl:allValuesFrom xsd:string
                            ] ,
                            [ rdf:type owl:Restriction ;
                              owl:onProperty :enum ;
                              owl:allValuesFrom rdfs:Literal
                            ] ;
            
            rdfs:comment "Any JSON value specification."@en .



###  http://www.w3.org/ns/td#Event

:Event rdf:type owl:Class ;
       
       rdfs:label "Event" ;
       
       rdfs:comment "The Event Interaction Pattern describes event sources that asynchronously push messages. Here not state, but state transitions (events) are communicated (e.g., \"clicked\"). Events may be triggered by internal state changes that are not exposed as Properties. Events usually follow strong consistency, where messages need to be queued to ensure eventual delivery of all occured events."@en .



###  http://www.w3.org/ns/td#Form

:Form rdf:type owl:Class ;
      
      rdfs:label "Form" ;
      
      rdfs:subClassOf [ rdf:type owl:Restriction ;
                        owl:onProperty :rel ;
                        owl:allValuesFrom xsd:string
                      ] ,
                      [ rdf:type owl:Restriction ;
                        owl:onProperty :mediaType ;
                        owl:allValuesFrom xsd:string
                      ] ,
                      [ rdf:type owl:Restriction ;
                        owl:onProperty :security ;
                        owl:allValuesFrom xsd:string
                      ] ,
                      [ rdf:type owl:Restriction ;
                        owl:onProperty :scopes ;
                        owl:allValuesFrom xsd:string
                      ] ,
                      [ rdf:type owl:Restriction ;
                        owl:onProperty :href ;
                        owl:someValuesFrom xsd:anyURI
                      ] ;
      
      rdfs:comment "Communication metadata indicating where a service can be accessed by a client application. An interaction might have more than one form."@en .



###  http://www.w3.org/ns/td#IntegerSchema

:IntegerSchema rdf:type owl:Class ;
               
               rdfs:subClassOf :NumberSchema ;
               
               rdfs:comment "A JSON integer value specification, i.e. numbers without a fractional part (\"type\": \"integer\")."@en .



###  http://www.w3.org/ns/td#Link

:Link rdf:type owl:Class ;
      
      rdfs:label "Link" ;
      
      rdfs:subClassOf [ rdf:type owl:Restriction ;
                        owl:onProperty :anchor ;
                        owl:allValuesFrom xsd:anyURI
                      ] ,
                      [ rdf:type owl:Restriction ;
                        owl:onProperty :href ;
                        owl:someValuesFrom xsd:anyURI
                      ] ,
                      [ rdf:type owl:Restriction ;
                        owl:onProperty :mediaType ;
                        owl:allValuesFrom xsd:string
                      ] ,
                      [ rdf:type owl:Restriction ;
                        owl:onProperty :rel ;
                        owl:allValuesFrom xsd:string
                      ] ;
      
      rdfs:comment "A Web link, as specified by IETF RFC 8288 (https://tools.ietf.org/html/rfc8288)."@en .



###  http://www.w3.org/ns/td#NumberSchema

:NumberSchema rdf:type owl:Class ;
              
              rdfs:subClassOf :DataSchema ,
                              [ rdf:type owl:Restriction ;
                                owl:onProperty :maximum ;
                                owl:allValuesFrom [ rdf:type rdfs:Datatype ;
                                                    owl:unionOf ( xsd:double
                                                                  xsd:integer
                                                                )
                                                  ]
                              ] ,
                              [ rdf:type owl:Restriction ;
                                owl:onProperty :minimum ;
                                owl:allValuesFrom [ rdf:type rdfs:Datatype ;
                                                    owl:unionOf ( xsd:double
                                                                  xsd:integer
                                                                )
                                                  ]
                              ] ;
              
              rdfs:comment "A JSON number value specification (\"type\": \"number\")."@en .



###  http://www.w3.org/ns/td#ObjectSchema

:ObjectSchema rdf:type owl:Class ;
              
              rdfs:subClassOf :DataSchema ,
                              [ rdf:type owl:Restriction ;
                                owl:onProperty :required ;
                                owl:allValuesFrom xsd:string
                              ] ,
                              [ rdf:type owl:Restriction ;
                                owl:onProperty :properties ;
                                owl:allValuesFrom :DataSchema
                              ] ;
              
              rdfs:comment "A JSON object specification (\"type\": \"object\")."@en .



###  http://www.w3.org/ns/td#Property

:Property rdf:type owl:Class ;
          
          rdfs:label "Property" ;
          
          rdfs:subClassOf [ rdf:type owl:Restriction ;
                            owl:onProperty :observable ;
                            owl:allValuesFrom xsd:boolean
                          ] ,
                          [ rdf:type owl:Restriction ;
                            owl:onProperty :forms ;
                            owl:allValuesFrom :Form
                          ] ,
                          [ rdf:type owl:Restriction ;
                            owl:onProperty :schema ;
                            owl:allValuesFrom :DataSchema
                          ] ,
                          [ rdf:type owl:Restriction ;
                            owl:onProperty :security ;
                            owl:allValuesFrom :SecurityScheme
                          ] ,
                          [ rdf:type owl:Restriction ;
                            owl:onProperty :scopes ;
                            owl:allValuesFrom xsd:string
                          ] ,
                          [ rdf:type owl:Restriction ;
                            owl:onProperty :writable ;
                            owl:allValuesFrom xsd:boolean
                          ] ,
                          [ rdf:type owl:Restriction ;
                            owl:onProperty :label ;
                            owl:allValuesFrom xsd:string
                          ] ;
          
          rdfs:comment "Properties expose internal state of a Thing that can be directly accessed (get) and optionally manipulated (set). In addition, Things can also choose to make Properties observable by pushing the new state (not an event) after a change; this must follow eventual consistency (also see CAP Theorem)."@en .

###  http://www.w3.org/ns/td#SecurityScheme

:SecurityScheme rdf:type owl:Class ;
          
          rdfs:label "SecurityScheme" ;

          rdfs:subClassOf [ rdf:type owl:Restriction ;
                            owl:onProperty :scheme ;
                            owl:allValuesFrom xsd:string
                          ] , 
                          [ rdf:type owl:Restriction ;
                            owl:onProperty :description ;
                            owl:allValuesFrom xsd:string
                          ] ,
                          [ rdf:type owl:Restriction ;
                            owl:onProperty :proxyUrl ;
                            owl:allValuesFrom xsd:anyURI
                          ] ; 
          
          rdfs:comment "An optional security configuration defines metadata for a security mechanism to allow access to one or more resources.  More than one security configuration may be specified in which case they all need to be satisfied for access to be permitted.  Security configurations can be given at the level of a Thing, an Interaction pattern, or a Form.  In this case security configurations given at lower levels override security configurations given at higher levels.  Additional security schemes can be used beyond those defined here if an appropriate external vocabulary is included in the context.  See also Security and Privacy Considerations."@en .
          


###  http://www.w3.org/ns/td#ArraySchema

:BasicSecurityScheme rdf:type owl:Class ;
             
             rdfs:subClassOf :SecurityScheme ;

             rdfs:subClassOf [ rdf:type owl:Restriction ;
                               owl:onProperty :in ;
                               owl:allValuesFrom xsd:string
                             ] , 
                             [ rdf:type owl:Restriction ;
                               owl:onProperty :pname ;
                               owl:allValuesFrom xsd:string
                             ] ; 
             
             rdfs:comment "Basic authentication security configuration (\"scheme\": \"basic\").  Unencrypted username and password.  Should be used with some other security mechanism providing confidentiality, for example, TLS."@en .

:DigestSecurityScheme rdf:type owl:Class ;
             
             rdfs:subClassOf :SecurityScheme ;

             rdfs:subClassOf [ rdf:type owl:Restriction ;
                               owl:onProperty :in ;
                               owl:allValuesFrom xsd:string
                             ] , 
                             [ rdf:type owl:Restriction ;
                               owl:onProperty :pname ;
                               owl:allValuesFrom xsd:string
                             ] , 
                             [ rdf:type owl:Restriction ;
                               owl:onProperty :qop ;
                               owl:allValuesFrom xsd:string
                             ] ; 
             
             rdfs:comment "Digest authentication security configuration (\"scheme\": \"digest\"). Similar to basic authentication but with added features to avoid man-in-the-middle attacks." .

:BearerSecurityScheme rdf:type owl:Class ;
             
             rdfs:subClassOf :SecurityScheme ;

             rdfs:subClassOf [ rdf:type owl:Restriction ;
                               owl:onProperty :alg ;
                               owl:allValuesFrom xsd:string
                             ] , 
                             [ rdf:type owl:Restriction ;
                               owl:onProperty :format ;
                               owl:allValuesFrom xsd:string
                             ] , 
                             [ rdf:type owl:Restriction ;
                               owl:onProperty :in ;
                               owl:allValuesFrom xsd:string
                             ] , 
                             [ rdf:type owl:Restriction ;
                               owl:onProperty :pname ;
                               owl:allValuesFrom xsd:string
                             ] , 
                             [ rdf:type owl:Restriction ;
                               owl:onProperty :authorizationUrl ;
                               owl:allValuesFrom xsd:anyURI
                             ] ; 

             rdfs:comment "Bearer token authentication security configuration (\"scheme\": \"bearer\").  This scheme is intended for situations where bearer tokens are used independently of OAuth.  If the oauth2 scheme is specified it is not generally necessary to specify this scheme as well as it is implied." .

:PopSecurityScheme rdf:type owl:Class ;
             
             rdfs:subClassOf :SecurityScheme ;

             rdfs:subClassOf [ rdf:type owl:Restriction ;
                               owl:onProperty :alg ;
                               owl:allValuesFrom xsd:string
                             ] , 
                             [ rdf:type owl:Restriction ;
                               owl:onProperty :format ;
                               owl:allValuesFrom xsd:string
                             ] , 
                             [ rdf:type owl:Restriction ;
                               owl:onProperty :in ;
                               owl:allValuesFrom xsd:string
                             ] , 
                             [ rdf:type owl:Restriction ;
                               owl:onProperty :pname ;
                               owl:allValuesFrom xsd:string
                             ] , 
                             [ rdf:type owl:Restriction ;
                               owl:onProperty :authorizationUrl ;
                               owl:allValuesFrom xsd:anyURI
                             ] ; 

             rdfs:comment "Proof-of-possession token authentication security configuration (\"scheme\": \"pop\")." .

:ApikeySecurityScheme rdf:type owl:Class ;
             
             rdfs:subClassOf :SecurityScheme ;

             rdfs:subClassOf [ rdf:type owl:Restriction ;
                               owl:onProperty :in ;
                               owl:allValuesFrom xsd:string
                             ] , 
                             [ rdf:type owl:Restriction ;
                               owl:onProperty :pname ;
                               owl:allValuesFrom xsd:string
                             ] ; 

             rdfs:comment "API key authentication security configuration (\"scheme\": \"apikey\").  This is for the case where the access token is opaque and is not using a standard token format."@en .

:OAuth2SecurityScheme rdf:type owl:Class ;
             
             rdfs:subClassOf :SecurityScheme ;

             rdfs:subClassOf [ rdf:type owl:Restriction ;
                               owl:onProperty :flow ;
                               owl:allValuesFrom xsd:string
                             ] , 
                             ### NOTE!  This is an (array) of strings, not objects; 
			     ### it would be nice to have descriptions, but would complicate the defn
                             [ rdf:type owl:Restriction ;
                               owl:onProperty :scopes ;
                               owl:allValuesFrom xsd:string
                             ] , 
                             [ rdf:type owl:Restriction ;
                               owl:onProperty :tokenUrl ;
                               owl:allValuesFrom xsd:anyURI
                             ] , 
                             [ rdf:type owl:Restriction ;
                               owl:onProperty :authorizationUrl ;
                               owl:allValuesFrom xsd:anyURI
                             ] , 
                             [ rdf:type owl:Restriction ;
                               owl:onProperty :refreshUrl ;
                               owl:allValuesFrom xsd:anyURI
                             ] ; 

             rdfs:comment "OAuth2 authentication security configuration (\"scheme\": \"oauth2\").  For the implicit flow the authorizationUrl and scopes are required.  For the password and client flows both tokenUrl and scopes are required.  For the code flow authorizationUrl, tokenUrl, and scopes are required."@en .
                  

###  http://www.w3.org/ns/td#SimpleDataSchema

:SimpleDataSchema rdf:type owl:Class ;
                  
                  owl:equivalentClass [ rdf:type owl:Class ;
                                        owl:unionOf ( :BooleanSchema
                                                      :NumberSchema
                                                      :StringSchema
                                                    )
                                      ] ;
                  
                  rdfs:subClassOf :DataSchema ;
                  
                  rdfs:seeAlso <http://schema.org/PropertyValueSpecification> .



###  http://www.w3.org/ns/td#StringSchema

:StringSchema rdf:type owl:Class ;
              
              rdfs:subClassOf :DataSchema ;
              
              rdfs:comment "A JSON string value specification (\"type\": \"string\")."@en .



###  http://www.w3.org/ns/td#Thing

:Thing rdf:type owl:Class ;
       
       rdfs:label "Thing"@en ;
       
       rdfs:subClassOf [ rdf:type owl:Restriction ;
                         owl:onProperty :name ;
                         owl:someValuesFrom xsd:string
                       ] ,
                       [ rdf:type owl:Restriction ;
                         owl:onProperty :base ;
                         owl:allValuesFrom xsd:anyURI
                       ] ,
                       [ rdf:type owl:Restriction ;
                         owl:onProperty :links ;
                         owl:allValuesFrom :Link
                       ] ,
                       [ rdf:type owl:Restriction ;
                         owl:onProperty :security ;
                         owl:allValuesFrom :Security
                       ] ,
                       [ rdf:type owl:Restriction ;
                         owl:onProperty :events ;
                         owl:allValuesFrom :Property
                       ] ,
                       [ rdf:type owl:Restriction ;
                         owl:onProperty :id ;
                         owl:allValuesFrom xsd:string
                       ] ,
                       [ rdf:type owl:Restriction ;
                         owl:onProperty :actions ;
                         owl:allValuesFrom :Action
                       ] ,
                       [ rdf:type owl:Restriction ;
                         owl:onProperty :support ;
                         owl:allValuesFrom xsd:string
                       ] ,
                       [ rdf:type owl:Restriction ;
                         owl:onProperty :description ;
                         owl:allValuesFrom xsd:string
                       ] ;
       
       rdfs:comment "Describes a physical and/or virtual Thing (may represent one or more physical and / or virtual Things) in the Web of Things context."@en .




###  Generated by the OWL API (version 3.4.2) http://owlapi.sourceforge.net

